src/library/constants.cpp
@@ -172,6 +172,7 @@ name const * g_mul = nullptr;
 name const * g_mul_one = nullptr;
 name const * g_mul_zero = nullptr;
 name const * g_mul_zero_class = nullptr;
+name const * g_name = nullptr;
 name const * g_name_anonymous = nullptr;
 name const * g_name_mk_string = nullptr;
 name const * g_nat = nullptr;
@@ -535,6 +536,7 @@ void initialize_constants() {
     g_mul_one = new name{"mul_one"};
     g_mul_zero = new name{"mul_zero"};
     g_mul_zero_class = new name{"mul_zero_class"};
+    g_name = new name{"name"};
     g_name_anonymous = new name{"name", "anonymous"};
     g_name_mk_string = new name{"name", "mk_string"};
     g_nat = new name{"nat"};
@@ -899,6 +901,7 @@ void finalize_constants() {
     delete g_mul_one;
     delete g_mul_zero;
     delete g_mul_zero_class;
+    delete g_name;
     delete g_name_anonymous;
     delete g_name_mk_string;
     delete g_nat;
@@ -1262,6 +1265,7 @@ name const & get_mul_name() { return *g_mul; }
 name const & get_mul_one_name() { return *g_mul_one; }
 name const & get_mul_zero_name() { return *g_mul_zero; }
 name const & get_mul_zero_class_name() { return *g_mul_zero_class; }
+name const & get_name_name() { return *g_name; }
 name const & get_name_anonymous_name() { return *g_name_anonymous; }
 name const & get_name_mk_string_name() { return *g_name_mk_string; }
 name const & get_nat_name() { return *g_nat; }
