src/library/constants.h
@@ -174,6 +174,7 @@ name const & get_mul_name();
 name const & get_mul_one_name();
 name const & get_mul_zero_name();
 name const & get_mul_zero_class_name();
+name const & get_name_name();
 name const & get_name_anonymous_name();
 name const & get_name_mk_string_name();
 name const & get_nat_name();
